io/Compiler.Model2.fst
@@ -129,6 +129,18 @@ let compile_pprog #i p_s =
   let eff_rcs = make_rcs_eff i.spt_rcs in
   (i.spt_exportable AllActions).export eff_rcs (p_s #AllActions)
 
+val compile_ctx : (#i:src_interface) -> (c_s:ctx_src i) -> ctx_tgt (comp_int_src_tgt i)
+let compile_ctx #i c_s =
+  (** TODO: the partial program should be also importable besides exportable,
+      which would be a pain because one has to define a second tree of rcs. **)
+
+  (** The point of defining C↓ is to prove SCC (from Beyond Full Abstraction). 
+      Since, C↓ = fun p -> C (import p) and P↓ = export P,
+      then C↓[P↓] = C↓ (P↓) = C↓ (export P) = C (import (export P)) = C P.
+      The last step is true if we can prove that `import (export f) = f`, see
+      LawImportableExportable.fst **)
+  admit ()
+
 let comp : compiler = {
   source = src_language;
   target = tgt_language;
